src/MicroSail/SmallStep/Inversion.v
@@ -72,8 +72,8 @@ Module Inversion
              => specialize (H _ _ _ eq_refl)
            | [ H : Final ?s -> _, H' : Final ?s |- _ ]
              => specialize (H H')
-           | [ H1 : ⟨ ?δ1, ?s1 ⟩ ---> ⟨ ?δ2, ?s2 ⟩,
-               H2 : ⟨ ?δ2, ?s2 ⟩ --->* ⟨ ?δ3, ?s3 ⟩ |- _ ]
+           | [ H1 : ⟨ _, _, _ ⟩ ---> ⟨ ?γ2, ?δ2, ?s2 ⟩,
+               H2 : ⟨ ?γ2, ?δ2, ?s2 ⟩ --->* ⟨ _, _, _ ⟩ |- _ ]
              => extend (step_trans H1 H2)
            end;
        steps_inversion_simpl).
@@ -84,88 +84,94 @@ Module Inversion
        | [ |- exists t, _ ] => eexists
        | [ |- _ /\ _ ] => constructor
        | [ |- True ] => constructor
-       | [ |- ⟨ _ , stm_lit _ _ ⟩ --->* ⟨ _, _ ⟩ ] => constructor 1
-       | [ |- ⟨ _ , stm_fail _ _ ⟩ --->* ⟨ _, _ ⟩ ] => constructor 1
-       | [ |- ⟨ _ , stm_let _ _ (stm_lit _ _) _ ⟩ ---> ⟨ _ , _ ⟩ ] => apply step_stm_let_value
-       | [ |- ⟨ _ , stm_let _ _ (stm_fail _ _) _ ⟩ ---> ⟨ _ , _ ⟩ ] => apply step_stm_let_fail
-       | [ |- ⟨ _ , stm_assign _ (stm_lit _ _) _ ⟩ ---> ⟨ _ , _ ⟩ ] => apply step_stm_assign_value
-       | [ |- ⟨ _ , stm_assign _ (stm_fail _ _) _ ⟩ ---> ⟨ _ , _ ⟩ ] => apply step_stm_assign_fail
+       | [ |- ⟨ _, _, stm_lit _ _ ⟩ --->* ⟨ _, _, _ ⟩ ] => constructor 1
+       | [ |- ⟨ _, _, stm_fail _ _ ⟩ --->* ⟨ _, _, _ ⟩ ] => constructor 1
+       | [ |- ⟨ _, _, stm_let _ _ (stm_lit _ _) _ ⟩ ---> ⟨ _, _, _ ⟩ ] => apply step_stm_let_value
+       | [ |- ⟨ _, _, stm_let _ _ (stm_fail _ _) _ ⟩ ---> ⟨ _, _, _ ⟩ ] => apply step_stm_let_fail
+       | [ |- ⟨ _, _, stm_assign _ (stm_lit _ _) _ ⟩ ---> ⟨ _, _, _ ⟩ ] => apply step_stm_assign_value
+       | [ |- ⟨ _, _, stm_assign _ (stm_fail _ _) _ ⟩ ---> ⟨ _, _, _ ⟩ ] => apply step_stm_assign_fail
        end; cbn); try eassumption.
 
   Local Ltac steps_inversion_induction :=
     let step := fresh in
-    induction 1 as [|? ? ? ? ? ? step]; intros; subst;
+    induction 1 as [|? ? ? ? ? ? ? ? ? step]; intros; subst;
       [ cbn in *; contradiction
       | inversion step; steps_inversion_inster; steps_inversion_solve
       ].
 
-  Lemma steps_inversion_let {Γ x τ σ} {δ1 δ3 : LocalStore Γ}
+  Lemma steps_inversion_let {Γ x τ σ} {γ1 γ3 : RegStore} {δ1 δ3 : LocalStore Γ}
     {s1 : Stm Γ τ} {s2 : Stm (ctx_snoc Γ (x, τ)) σ} {t : Stm Γ σ} (final : Final t)
-    (steps : ⟨ δ1, stm_let x τ s1 s2 ⟩ --->* ⟨ δ3, t ⟩) :
-    exists (δ2 : LocalStore Γ) (s1' : Stm Γ τ),
-    (⟨ δ1, s1 ⟩ --->* ⟨ δ2, s1' ⟩) /\ Final s1' /\
-    (exists (s0 : Stm Γ σ),
-        (⟨ δ2, stm_let x τ s1' s2 ⟩ ---> ⟨ δ2, s0 ⟩) /\ ⟨ δ2, s0 ⟩ --->* ⟨ δ3, t ⟩).
+    (steps : ⟨ γ1, δ1, stm_let x τ s1 s2 ⟩ --->* ⟨ γ3, δ3, t ⟩) :
+    exists (γ2 : RegStore) (δ2 : LocalStore Γ) (s1' : Stm Γ τ),
+      ⟨ γ1, δ1, s1 ⟩ --->* ⟨ γ2, δ2, s1' ⟩ /\ Final s1' /\
+      exists (s0 : Stm Γ σ),
+          ⟨ γ2, δ2, stm_let x τ s1' s2 ⟩ ---> ⟨ γ2, δ2, s0 ⟩ /\
+          ⟨ γ2, δ2, s0 ⟩ --->* ⟨ γ3, δ3, t ⟩.
   Proof.
     remember (stm_let x τ s1 s2) as s. revert steps s1 s2 Heqs.
     steps_inversion_induction.
   Qed.
 
-  Lemma steps_inversion_let' {Γ Δ σ} (δ1 δ3 : LocalStore Γ)
-    (δΔ : LocalStore Δ) (k : Stm (ctx_cat Γ Δ) σ) (t : Stm Γ σ) (final : Final t)
-    (steps : ⟨ δ1, stm_let' δΔ k ⟩ --->* ⟨ δ3, t ⟩) :
-    exists δ2 δΔ' k',
-      ⟨ env_cat δ1 δΔ , k ⟩ --->* ⟨ env_cat δ2 δΔ' , k' ⟩ /\ Final k' /\
+  Lemma steps_inversion_let' {Γ Δ σ} {γ1 γ3 : RegStore} {δ1 δ3 : LocalStore Γ}
+    {δΔ : LocalStore Δ} {k : Stm (ctx_cat Γ Δ) σ} {t : Stm Γ σ} (final : Final t)
+    (steps : ⟨ γ1, δ1, stm_let' δΔ k ⟩ --->* ⟨ γ3, δ3, t ⟩) :
+    exists γ2 δ2 δΔ' k',
+      ⟨ γ1, env_cat δ1 δΔ , k ⟩ --->* ⟨ γ2, env_cat δ2 δΔ' , k' ⟩ /\ Final k' /\
       exists (s0 : Stm Γ σ),
-        (⟨ δ2, stm_let' δΔ' k' ⟩ ---> ⟨ δ2, s0 ⟩) /\ (⟨ δ2, s0 ⟩ --->* ⟨ δ3, t ⟩).
+        ⟨ γ2, δ2, stm_let' δΔ' k' ⟩ ---> ⟨ γ2, δ2, s0 ⟩ /\
+        ⟨ γ2, δ2, s0 ⟩ --->* ⟨ γ3, δ3, t ⟩.
   Proof.
     remember (stm_let' δΔ k) as s. revert steps δΔ k Heqs.
     steps_inversion_induction.
   Qed.
 
-  Lemma steps_inversion_seq {Γ τ σ} (δ1 δ3 : LocalStore Γ)
+  Lemma steps_inversion_seq {Γ τ σ} {γ1 γ3 : RegStore} {δ1 δ3 : LocalStore Γ}
     (s1 : Stm Γ τ) (s2 : Stm Γ σ) (t : Stm Γ σ) (final : Final t)
-    (steps : ⟨ δ1, stm_seq s1 s2 ⟩ --->* ⟨ δ3, t ⟩) :
-    exists δ2 s1',
-      ⟨ δ1, s1 ⟩ --->* ⟨ δ2, s1' ⟩ /\ Final s1' /\
+    (steps : ⟨ γ1, δ1, stm_seq s1 s2 ⟩ --->* ⟨ γ3, δ3, t ⟩) :
+    exists γ2 δ2 s1',
+      ⟨ γ1, δ1, s1 ⟩ --->* ⟨ γ2, δ2, s1' ⟩ /\ Final s1' /\
       exists (s0 : Stm Γ σ),
-        (⟨ δ2, stm_seq s1' s2 ⟩ ---> ⟨ δ2 , s0 ⟩) /\ (⟨ δ2 , s0 ⟩ --->* ⟨ δ3, t ⟩).
+        ⟨ γ2, δ2, stm_seq s1' s2 ⟩ ---> ⟨ γ2, δ2 , s0 ⟩ /\
+        ⟨ γ2, δ2 , s0 ⟩ --->* ⟨ γ3, δ3, t ⟩.
   Proof.
     remember (stm_seq s1 s2) as s. revert steps s1 s2 Heqs.
     steps_inversion_induction.
   Qed.
 
-  Lemma steps_inversion_call' {Γ Δ σ} (δ1 δ3 : LocalStore Γ)
+  Lemma steps_inversion_call' {Γ Δ σ} {γ1 γ3 : RegStore} {δ1 δ3 : LocalStore Γ}
     (δΔ : LocalStore Δ) (k : Stm Δ σ) (t : Stm Γ σ) (final : Final t)
-    (steps : ⟨ δ1, stm_call' Δ δΔ σ k ⟩ --->* ⟨ δ3, t ⟩) :
-    exists δΔ' k',
-      ⟨ δΔ , k ⟩ --->* ⟨ δΔ' , k' ⟩ /\ Final k' /\
+    (steps : ⟨ γ1, δ1, stm_call' Δ δΔ σ k ⟩ --->* ⟨ γ3, δ3, t ⟩) :
+    exists γ2 δΔ' k',
+      ⟨ γ1, δΔ , k ⟩ --->* ⟨ γ2, δΔ' , k' ⟩ /\ Final k' /\
       exists s0,
-      (⟨ δ1, stm_call' Δ δΔ' σ k' ⟩ ---> ⟨ δ1, s0 ⟩) /\ (⟨ δ1, s0⟩ --->* ⟨ δ3, t ⟩).
+        ⟨ γ2, δ1, stm_call' Δ δΔ' σ k' ⟩ ---> ⟨ γ2, δ1, s0 ⟩ /\
+        ⟨ γ2, δ1, s0⟩ --->* ⟨ γ3, δ3, t ⟩.
   Proof.
     remember (stm_call' Δ δΔ σ k) as s. revert steps δΔ k Heqs.
     steps_inversion_induction.
   Qed.
 
-  Lemma steps_inversion_assign {Γ σ} (δ1 δ3 : LocalStore Γ)
+  Lemma steps_inversion_assign {Γ σ} {γ1 γ3 : RegStore} {δ1 δ3 : LocalStore Γ}
     (x : 𝑿) (xInΓ : InCtx (x,σ) Γ) (s1 t : Stm Γ σ) (final : Final t)
-    (steps : ⟨ δ1, stm_assign x s1 ⟩ --->* ⟨ δ3, t ⟩) :
-    exists δ2 δ2' s1',
-      ⟨ δ1, s1 ⟩ --->* ⟨ δ2, s1' ⟩ /\ Final s1' /\
+    (steps : ⟨ γ1, δ1, stm_assign x s1 ⟩ --->* ⟨ γ3, δ3, t ⟩) :
+    exists γ2 δ2 δ2' s1',
+      ⟨ γ1, δ1, s1 ⟩ --->* ⟨ γ2, δ2, s1' ⟩ /\ Final s1' /\
       exists (s0 : Stm Γ σ),
-        (⟨ δ2, stm_assign x s1' ⟩ ---> ⟨ δ2' , s0 ⟩) /\ (⟨ δ2' , s0 ⟩ --->* ⟨ δ3, t ⟩).
+        ⟨ γ2, δ2, stm_assign x s1' ⟩ ---> ⟨ γ2, δ2' , s0 ⟩ /\
+        ⟨ γ2, δ2' , s0 ⟩ --->* ⟨ γ3, δ3, t ⟩.
   Proof.
     remember (stm_assign x s1) as s. revert steps x xInΓ s1 Heqs.
     steps_inversion_induction.
   Qed.
 
-  Lemma steps_inversion_bind {Γ τ σ} (δ1 δ3 : LocalStore Γ)
+  Lemma steps_inversion_bind {Γ τ σ} {γ1 γ3 : RegStore} {δ1 δ3 : LocalStore Γ}
     (s1 : Stm Γ τ) (k : Lit τ -> Stm Γ σ) (t : Stm Γ σ) (final : Final t)
-    (steps : ⟨ δ1, stm_bind s1 k ⟩ --->* ⟨ δ3, t ⟩) :
-    exists δ2 s1',
-      ⟨ δ1, s1 ⟩ --->* ⟨ δ2, s1' ⟩ /\ Final s1' /\
+    (steps : ⟨ γ1, δ1, stm_bind s1 k ⟩ --->* ⟨ γ3, δ3, t ⟩) :
+    exists γ2 δ2 s1',
+      ⟨ γ1, δ1, s1 ⟩ --->* ⟨ γ2, δ2, s1' ⟩ /\ Final s1' /\
       exists (s0 : Stm Γ σ),
-        (⟨ δ2, stm_bind s1' k ⟩ ---> ⟨ δ2 , s0 ⟩) /\ (⟨ δ2 , s0 ⟩ --->* ⟨ δ3, t ⟩).
+        ⟨ γ2, δ2, stm_bind s1' k ⟩ ---> ⟨ γ2, δ2 , s0 ⟩ /\
+        ⟨ γ2, δ2 , s0 ⟩ --->* ⟨ γ3, δ3, t ⟩.
   Proof.
     remember (stm_bind s1 k) as s. revert steps s1 k Heqs.
     steps_inversion_induction.
