src/MicroSail/SmallStep/Step.v
@@ -41,154 +41,157 @@ Module SmallStep
   Import CtxNotations.
   Import EnvNotations.
 
-  Inductive Step {Γ : Ctx (𝑿 * Ty)} : forall {σ : Ty} (δ1 δ2 : LocalStore Γ) (s1 s2 : Stm Γ σ), Prop :=
+  Inductive Step {Γ : Ctx (𝑿 * Ty)} : forall {σ : Ty} (γ1 γ2 : RegStore) (δ1 δ2 : LocalStore Γ) (s1 s2 : Stm Γ σ), Prop :=
 
   | step_stm_exp
-      (δ : LocalStore Γ) (σ : Ty) (e : Exp Γ σ) :
-      ⟨ δ , stm_exp e ⟩ ---> ⟨ δ , stm_lit σ (eval e δ) ⟩
+      (γ : RegStore) (δ : LocalStore Γ) (σ : Ty) (e : Exp Γ σ) :
+      ⟨ γ , δ , stm_exp e ⟩ ---> ⟨ γ , δ , stm_lit σ (eval e δ) ⟩
 
   | step_stm_let_value
-      (δ : LocalStore Γ) (x : 𝑿) (τ σ : Ty) (v : Lit τ) (k : Stm (Γ ▻ (x , τ)) σ) :
-      ⟨ δ , stm_let x τ (stm_lit τ v) k ⟩ ---> ⟨ δ , stm_let' (env_snoc env_nil (x,τ) v) k ⟩
+      (γ : RegStore) (δ : LocalStore Γ) (x : 𝑿) (τ σ : Ty) (v : Lit τ) (k : Stm (Γ ▻ (x , τ)) σ) :
+      ⟨ γ , δ , stm_let x τ (stm_lit τ v) k ⟩ ---> ⟨ γ , δ , stm_let' (env_snoc env_nil (x,τ) v) k ⟩
   | step_stm_let_fail
-      (δ : LocalStore Γ) (x : 𝑿) (τ σ : Ty) (s : string) (k : Stm (Γ ▻ (x , τ)) σ) :
-      ⟨ δ , stm_let x τ (stm_fail τ s) k ⟩ ---> ⟨ δ , stm_fail σ s ⟩
+      (γ : RegStore) (δ : LocalStore Γ) (x : 𝑿) (τ σ : Ty) (s : string) (k : Stm (Γ ▻ (x , τ)) σ) :
+      ⟨ γ , δ , stm_let x τ (stm_fail τ s) k ⟩ ---> ⟨ γ , δ , stm_fail σ s ⟩
   | step_stm_let_step
-      (δ : LocalStore Γ) (δ' : LocalStore Γ) (x : 𝑿) (τ σ : Ty)
+      (γ γ' : RegStore) (δ δ' : LocalStore Γ) (x : 𝑿) (τ σ : Ty)
       (s : Stm Γ τ) (s' : Stm Γ τ) (k : Stm (Γ ▻ (x , τ)) σ) :
-      ⟨ δ , s ⟩ ---> ⟨ δ' , s' ⟩ ->
-      ⟨ δ , stm_let x τ s k ⟩ ---> ⟨ δ' , stm_let x τ s' k ⟩
+      ⟨ γ , δ , s ⟩ ---> ⟨ γ' , δ' , s' ⟩ ->
+      ⟨ γ , δ , stm_let x τ s k ⟩ ---> ⟨ γ', δ' , stm_let x τ s' k ⟩
   | step_stm_let'_value
-      (δ : LocalStore Γ) (Δ : Ctx (𝑿 * Ty)) (δΔ : LocalStore Δ) (σ : Ty) (v : Lit σ) :
-      ⟨ δ , stm_let' δΔ (stm_lit σ v) ⟩ ---> ⟨ δ , stm_lit σ v ⟩
+      (γ : RegStore) (δ : LocalStore Γ) (Δ : Ctx (𝑿 * Ty)) (δΔ : LocalStore Δ) (σ : Ty) (v : Lit σ) :
+      ⟨ γ , δ , stm_let' δΔ (stm_lit σ v) ⟩ ---> ⟨ γ , δ , stm_lit σ v ⟩
   | step_stm_let'_fail
-      (δ : LocalStore Γ) (Δ : Ctx (𝑿 * Ty)) (δΔ : LocalStore Δ) (σ : Ty) (s : string) :
-      ⟨ δ , stm_let' δΔ (stm_fail σ s) ⟩ ---> ⟨ δ , stm_fail σ s ⟩
+      (γ : RegStore) (δ : LocalStore Γ) (Δ : Ctx (𝑿 * Ty)) (δΔ : LocalStore Δ) (σ : Ty) (s : string) :
+      ⟨ γ , δ , stm_let' δΔ (stm_fail σ s) ⟩ ---> ⟨ γ , δ , stm_fail σ s ⟩
   | step_stm_let'_step
-      (δ δ' : LocalStore Γ) (Δ : Ctx (𝑿 * Ty)) (δΔ δΔ' : LocalStore Δ) (σ : Ty) (k k' : Stm (Γ ▻▻ Δ) σ) :
-      ⟨ δ ►► δΔ , k ⟩ ---> ⟨ δ' ►► δΔ' , k' ⟩ ->
-      ⟨ δ , stm_let' δΔ k ⟩ ---> ⟨ δ' , stm_let' δΔ' k' ⟩
+      (γ γ' : RegStore) (δ δ' : LocalStore Γ) (Δ : Ctx (𝑿 * Ty)) (δΔ δΔ' : LocalStore Δ) (σ : Ty) (k k' : Stm (Γ ▻▻ Δ) σ) :
+      ⟨ γ , δ ►► δΔ , k ⟩ ---> ⟨ γ', δ' ►► δΔ' , k' ⟩ ->
+      ⟨ γ , δ , stm_let' δΔ k ⟩ ---> ⟨ γ' , δ' , stm_let' δΔ' k' ⟩
 
   | step_stm_seq_step
-      (δ δ' : LocalStore Γ) (τ σ : Ty) (s s' : Stm Γ τ) (k : Stm Γ σ) :
-      ⟨ δ , s ⟩ ---> ⟨ δ' , s' ⟩ ->
-      ⟨ δ , stm_seq s k ⟩ ---> ⟨ δ' , stm_seq s' k ⟩
+      (γ γ' : RegStore) (δ δ' : LocalStore Γ) (τ σ : Ty) (s s' : Stm Γ τ) (k : Stm Γ σ) :
+      ⟨ γ , δ , s ⟩ ---> ⟨ γ' , δ' , s' ⟩ ->
+      ⟨ γ , δ , stm_seq s k ⟩ ---> ⟨ γ', δ' , stm_seq s' k ⟩
   | step_stm_seq_value
-      (δ : LocalStore Γ) (τ σ : Ty) (v : Lit τ) (k : Stm Γ σ) :
-      ⟨ δ , stm_seq (stm_lit τ v) k ⟩ ---> ⟨ δ , k ⟩
+      (γ : RegStore) (δ : LocalStore Γ) (τ σ : Ty) (v : Lit τ) (k : Stm Γ σ) :
+      ⟨ γ , δ , stm_seq (stm_lit τ v) k ⟩ ---> ⟨ γ , δ , k ⟩
   | step_stm_seq_fail
-      (δ : LocalStore Γ) (τ σ : Ty) (s : string) (k : Stm Γ σ) :
-      ⟨ δ , stm_seq (stm_fail τ s) k ⟩ ---> ⟨ δ , stm_fail σ s ⟩
+      (γ : RegStore) (δ : LocalStore Γ) (τ σ : Ty) (s : string) (k : Stm Γ σ) :
+      ⟨ γ , δ , stm_seq (stm_fail τ s) k ⟩ ---> ⟨ γ , δ , stm_fail σ s ⟩
 
   | step_stm_call
-      {δ : LocalStore Γ} {σs σ} {f : 𝑭 σs σ} (es : Env' (Exp Γ) σs) :
-      ⟨ δ , stm_call f es ⟩ --->
-      ⟨ δ , stm_call' σs (evals es δ) σ (Pi f) ⟩
+      (γ : RegStore) (δ : LocalStore Γ) {σs σ} {f : 𝑭 σs σ} (es : Env' (Exp Γ) σs) :
+      ⟨ γ , δ , stm_call f es ⟩ --->
+      ⟨ γ , δ , stm_call' σs (evals es δ) σ (Pi f) ⟩
   | step_stm_call'_step
-      {δ : LocalStore Γ} (Δ : Ctx (𝑿 * Ty)) {δΔ δΔ' : LocalStore Δ} (τ : Ty)
+      (γ γ' : RegStore) (δ : LocalStore Γ) (Δ : Ctx (𝑿 * Ty)) {δΔ δΔ' : LocalStore Δ} (τ : Ty)
       (s s' : Stm Δ τ) :
-      ⟨ δΔ , s ⟩ ---> ⟨ δΔ' , s' ⟩ ->
-      ⟨ δ , stm_call' Δ δΔ τ s ⟩ ---> ⟨ δ , stm_call' Δ δΔ' τ s' ⟩
+      ⟨ γ , δΔ , s ⟩ ---> ⟨ γ' , δΔ' , s' ⟩ ->
+      ⟨ γ , δ , stm_call' Δ δΔ τ s ⟩ ---> ⟨ γ' , δ , stm_call' Δ δΔ' τ s' ⟩
   | step_stm_call'_value
-      {δ : LocalStore Γ} (Δ : Ctx (𝑿 * Ty)) {δΔ : LocalStore Δ} (τ : Ty) (v : Lit τ) :
-      ⟨ δ , stm_call' Δ δΔ τ (stm_lit τ v) ⟩ ---> ⟨ δ , stm_lit τ v ⟩
+      (γ : RegStore) (δ : LocalStore Γ) (Δ : Ctx (𝑿 * Ty)) {δΔ : LocalStore Δ} (τ : Ty) (v : Lit τ) :
+      ⟨ γ , δ , stm_call' Δ δΔ τ (stm_lit τ v) ⟩ ---> ⟨ γ , δ , stm_lit τ v ⟩
   | step_stm_call'_fail
-      {δ : LocalStore Γ} (Δ : Ctx (𝑿 * Ty)) {δΔ : LocalStore Δ} (τ : Ty) (s : string) :
-      ⟨ δ , stm_call' Δ δΔ τ (stm_fail τ s) ⟩ ---> ⟨ δ , stm_fail τ s ⟩
+      (γ : RegStore) (δ : LocalStore Γ) (Δ : Ctx (𝑿 * Ty)) {δΔ : LocalStore Δ} (τ : Ty) (s : string) :
+      ⟨ γ , δ , stm_call' Δ δΔ τ (stm_fail τ s) ⟩ ---> ⟨ γ , δ , stm_fail τ s ⟩
 
   | step_stm_assign_value
-      (δ : LocalStore Γ) (x : 𝑿) (σ : Ty) {xInΓ : InCtx (x , σ) Γ} (v : Lit σ) :
-      ⟨ δ , stm_assign x (stm_lit σ v) ⟩ ---> ⟨ δ ⟪ x ↦ v ⟫ , stm_lit σ v ⟩
+      (γ : RegStore) (δ : LocalStore Γ) (x : 𝑿) (σ : Ty) {xInΓ : InCtx (x , σ) Γ} (v : Lit σ) :
+      ⟨ γ , δ , stm_assign x (stm_lit σ v) ⟩ ---> ⟨ γ , δ ⟪ x ↦ v ⟫ , stm_lit σ v ⟩
   | step_stm_assign_fail
-      (δ : LocalStore Γ) (x : 𝑿) (σ : Ty) {xInΓ : InCtx (x , σ) Γ} (s : string) :
-      ⟨ δ , stm_assign x (stm_fail σ s) ⟩ ---> ⟨ δ , stm_fail σ s ⟩
+      (γ : RegStore) (δ : LocalStore Γ) (x : 𝑿) (σ : Ty) {xInΓ : InCtx (x , σ) Γ} (s : string) :
+      ⟨ γ , δ , stm_assign x (stm_fail σ s) ⟩ ---> ⟨ γ , δ , stm_fail σ s ⟩
   | step_stm_assign_step
-      (δ δ' : LocalStore Γ) (x : 𝑿) (σ : Ty) {xInΓ : InCtx (x , σ) Γ} (s s' : Stm Γ σ) :
-      ⟨ δ , s ⟩ ---> ⟨ δ' , s' ⟩ ->
-      ⟨ δ , stm_assign x s ⟩ ---> ⟨ δ' , stm_assign x s' ⟩
+      (γ γ' : RegStore) (δ δ' : LocalStore Γ) (x : 𝑿) (σ : Ty) {xInΓ : InCtx (x , σ) Γ} (s s' : Stm Γ σ) :
+      ⟨ γ , δ , s ⟩ ---> ⟨ γ' , δ' , s' ⟩ ->
+      ⟨ γ , δ , stm_assign x s ⟩ ---> ⟨ γ' , δ' , stm_assign x s' ⟩
 
   | step_stm_if
-      (δ : LocalStore Γ) (e : Exp Γ ty_bool) (σ : Ty) (s1 s2 : Stm Γ σ) :
-      ⟨ δ , stm_if e s1 s2 ⟩ ---> ⟨ δ , if eval e δ then s1 else s2 ⟩
+      (γ : RegStore) (δ : LocalStore Γ) (e : Exp Γ ty_bool) (σ : Ty) (s1 s2 : Stm Γ σ) :
+      ⟨ γ , δ , stm_if e s1 s2 ⟩ ---> ⟨ γ , δ , if eval e δ then s1 else s2 ⟩
   | step_stm_assert
-      (δ : LocalStore Γ) (e1 : Exp Γ ty_bool) (e2 : Exp Γ ty_string) :
-      ⟨ δ , stm_assert e1 e2 ⟩ --->
-      ⟨ δ , if eval e1 δ then stm_lit ty_bool true else stm_fail ty_bool (eval e2 δ) ⟩
-  (* | step_stm_while : *)
-  (*   (δ : LocalStore Γ) (w : 𝑾 δ) (e : Exp Γ ty_bool) {σ : Ty} (s : Stm Γ σ) -> *)
-  (*   ⟨ δ , stm_while w e s ⟩ ---> *)
-  (*   ⟨ δ , stm_if e (stm_seq s (stm_while w e s)) (stm_lit tt) ⟩ *)
+      (γ : RegStore) (δ : LocalStore Γ) (e1 : Exp Γ ty_bool) (e2 : Exp Γ ty_string) :
+      ⟨ γ , δ , stm_assert e1 e2 ⟩ --->
+      ⟨ γ , δ , if eval e1 δ then stm_lit ty_bool true else stm_fail ty_bool (eval e2 δ) ⟩
   | step_stm_match_list
-      (δ : LocalStore Γ) {σ τ : Ty} (e : Exp Γ (ty_list σ)) (alt_nil : Stm Γ τ)
+      (γ : RegStore) (δ : LocalStore Γ) {σ τ : Ty} (e : Exp Γ (ty_list σ)) (alt_nil : Stm Γ τ)
       (xh xt : 𝑿) (alt_cons : Stm (Γ ▻ (xh , σ) ▻ (xt , ty_list σ)) τ) :
-      ⟨ δ , stm_match_list e alt_nil xh xt alt_cons ⟩ --->
-      ⟨ δ , match eval e δ with
-            | nil => alt_nil
-            | cons vh vt => stm_let' (env_snoc (env_snoc env_nil (xh,σ) vh) (xt,ty_list σ) vt) alt_cons
-            end
+      ⟨ γ , δ , stm_match_list e alt_nil xh xt alt_cons ⟩ --->
+      ⟨ γ , δ , match eval e δ with
+                | nil => alt_nil
+                | cons vh vt => stm_let' (env_snoc (env_snoc env_nil (xh,σ) vh) (xt,ty_list σ) vt) alt_cons
+                end
       ⟩
   | step_stm_match_sum
-      (δ : LocalStore Γ) {σinl σinr τ : Ty} (e : Exp Γ (ty_sum σinl σinr))
+      (γ : RegStore) (δ : LocalStore Γ) {σinl σinr τ : Ty} (e : Exp Γ (ty_sum σinl σinr))
       (xinl : 𝑿) (alt_inl : Stm (Γ ▻ (xinl , σinl)) τ)
       (xinr : 𝑿) (alt_inr : Stm (Γ ▻ (xinr , σinr)) τ) :
-      ⟨ δ , stm_match_sum e xinl alt_inl xinr alt_inr ⟩ --->
-      ⟨ δ , match eval e δ with
-            | inl v => stm_let' (env_snoc env_nil (xinl,σinl) v) alt_inl
-            | inr v => stm_let' (env_snoc env_nil (xinr,σinr) v) alt_inr
-            end
+      ⟨ γ , δ , stm_match_sum e xinl alt_inl xinr alt_inr ⟩ --->
+      ⟨ γ , δ , match eval e δ with
+                | inl v => stm_let' (env_snoc env_nil (xinl,σinl) v) alt_inl
+                | inr v => stm_let' (env_snoc env_nil (xinr,σinr) v) alt_inr
+                end
       ⟩
   | step_stm_match_pair
-      (δ : LocalStore Γ) {σ1 σ2 τ : Ty} (e : Exp Γ (ty_prod σ1 σ2)) (xl xr : 𝑿)
+      (γ : RegStore) (δ : LocalStore Γ) {σ1 σ2 τ : Ty} (e : Exp Γ (ty_prod σ1 σ2)) (xl xr : 𝑿)
       (rhs : Stm (Γ ▻ (xl , σ1) ▻ (xr , σ2)) τ) :
-      ⟨ δ , stm_match_pair e xl xr rhs ⟩ --->
-      ⟨ δ , let (vl , vr) := eval e δ in
-            stm_let' (env_snoc (env_snoc env_nil (xl,σ1) vl) (xr,σ2) vr) rhs
+      ⟨ γ , δ , stm_match_pair e xl xr rhs ⟩ --->
+      ⟨ γ , δ , let (vl , vr) := eval e δ in
+                stm_let' (env_snoc (env_snoc env_nil (xl,σ1) vl) (xr,σ2) vr) rhs
       ⟩
   | step_stm_match_enum
-      (δ : LocalStore Γ) {E : 𝑬} (e : Exp Γ (ty_enum E)) {τ : Ty}
+      (γ : RegStore) (δ : LocalStore Γ) {E : 𝑬} (e : Exp Γ (ty_enum E)) {τ : Ty}
       (alts : forall (K : 𝑬𝑲 E), Stm Γ τ) :
-      ⟨ δ , stm_match_enum E e alts ⟩ ---> ⟨ δ , alts (eval e δ) ⟩
+      ⟨ γ , δ , stm_match_enum E e alts ⟩ ---> ⟨ γ , δ , alts (eval e δ) ⟩
   | step_stm_match_tuple
-      (δ : LocalStore Γ) {σs : Ctx Ty} {Δ : Ctx (𝑿 * Ty)}
+      (γ : RegStore) (δ : LocalStore Γ) {σs : Ctx Ty} {Δ : Ctx (𝑿 * Ty)}
       (e : Exp Γ (ty_tuple σs)) (p : TuplePat σs Δ)
       {τ : Ty} (rhs : Stm (ctx_cat Γ Δ) τ) :
-      ⟨ δ , stm_match_tuple e p rhs ⟩ --->
-      ⟨ δ , stm_let' (tuple_pattern_match p (eval e δ)) rhs ⟩
+      ⟨ γ , δ , stm_match_tuple e p rhs ⟩ --->
+      ⟨ γ , δ , stm_let' (tuple_pattern_match p (eval e δ)) rhs ⟩
 
   | step_stm_match_union
-      (δ : LocalStore Γ) {T : 𝑻} (e : Exp Γ (ty_union T)) {τ : Ty}
+      (γ : RegStore) (δ : LocalStore Γ) {T : 𝑻} (e : Exp Γ (ty_union T)) {τ : Ty}
       (altx : forall (K : 𝑲 T), 𝑿)
       (alts : forall (K : 𝑲 T), Stm (ctx_snoc Γ (altx K , 𝑲_Ty K)) τ) :
-      ⟨ δ , stm_match_union T e altx alts ⟩ --->
-      ⟨ δ , let (K , v) := eval e δ in
-            stm_let' (env_snoc env_nil (altx K,𝑲_Ty K) (untag v)) (alts K)
+      ⟨ γ , δ , stm_match_union T e altx alts ⟩ --->
+      ⟨ γ , δ , let (K , v) := eval e δ in
+                stm_let' (env_snoc env_nil (altx K,𝑲_Ty K) (untag v)) (alts K)
       ⟩
   | step_stm_match_record
-      (δ : LocalStore Γ) {R : 𝑹} {Δ : Ctx (𝑿 * Ty)}
+      (γ : RegStore) (δ : LocalStore Γ) {R : 𝑹} {Δ : Ctx (𝑿 * Ty)}
       (e : Exp Γ (ty_record R)) (p : RecordPat (𝑹𝑭_Ty R) Δ)
       {τ : Ty} (rhs : Stm (ctx_cat Γ Δ) τ) :
-      ⟨ δ , stm_match_record R e p rhs ⟩ --->
-      ⟨ δ , stm_let' (record_pattern_match p (eval e δ)) rhs ⟩
+      ⟨ γ , δ , stm_match_record R e p rhs ⟩ --->
+      ⟨ γ , δ , stm_let' (record_pattern_match p (eval e δ)) rhs ⟩
+
+  | step_stm_reg_register
+      (γ : RegStore) (δ : LocalStore Γ) {σ : Ty} (r : 𝑹𝑬𝑮 σ) :
+      ⟨ γ, δ, stm_read_register r ⟩ ---> ⟨ γ, δ, stm_lit σ (γ σ r) ⟩
+  | step_stm_write_register
+      (γ : RegStore) (δ : LocalStore Γ) {σ : Ty} (r : 𝑹𝑬𝑮 σ) (e : Exp Γ σ) :
+      let v := eval e δ in
+      ⟨ γ, δ, stm_write_register r e ⟩ ---> ⟨ write_register γ r v , δ , stm_lit σ v ⟩
 
   | step_stm_bind_step
-      (δ δ' : LocalStore Γ) (σ τ : Ty) (s s' : Stm Γ σ) (k : Lit σ -> Stm Γ τ) :
-      ⟨ δ , s ⟩ ---> ⟨ δ' , s' ⟩ ->
-      ⟨ δ , stm_bind s k ⟩ ---> ⟨ δ' , stm_bind s' k ⟩
+      (γ γ' : RegStore) (δ δ' : LocalStore Γ) (σ τ : Ty) (s s' : Stm Γ σ) (k : Lit σ -> Stm Γ τ) :
+      ⟨ γ , δ , s ⟩ ---> ⟨ γ', δ' , s' ⟩ ->
+      ⟨ γ , δ , stm_bind s k ⟩ ---> ⟨ γ', δ' , stm_bind s' k ⟩
   | step_stm_bind_value
-      (δ : LocalStore Γ) (σ τ : Ty) (v : Lit σ) (k : Lit σ -> Stm Γ τ) :
-      ⟨ δ , stm_bind (stm_lit σ v) k ⟩ ---> ⟨ δ , k v ⟩
+      (γ : RegStore) (δ : LocalStore Γ) (σ τ : Ty) (v : Lit σ) (k : Lit σ -> Stm Γ τ) :
+      ⟨ γ , δ , stm_bind (stm_lit σ v) k ⟩ ---> ⟨ γ , δ , k v ⟩
   | step_stm_bind_fail
-      (δ : LocalStore Γ) (σ τ : Ty) (s : string) (k : Lit σ -> Stm Γ τ) :
-      ⟨ δ , stm_bind (stm_fail σ s) k ⟩ ---> ⟨ δ , stm_fail τ s ⟩
+      (γ : RegStore) (δ : LocalStore Γ) (σ τ : Ty) (s : string) (k : Lit σ -> Stm Γ τ) :
+      ⟨ γ , δ , stm_bind (stm_fail σ s) k ⟩ ---> ⟨ γ , δ , stm_fail τ s ⟩
 
-  where "'⟨' δ1 ',' s1 '⟩' '--->' '⟨' δ2 ',' s2 '⟩'" := (@Step _ _ δ1%env δ2%env s1%stm s2%stm).
+  where "⟨ γ1 , δ1 , s1 ⟩ ---> ⟨ γ2 , δ2 , s2 ⟩" := (@Step _ _ γ1%env γ2%env δ1%env δ2%env s1%stm s2%stm).
 
-  Inductive Steps {Γ : Ctx (𝑿 * Ty)} {σ : Ty} (δ1 : LocalStore Γ) (s1 : Stm Γ σ) : LocalStore Γ -> Stm Γ σ -> Prop :=
-  | step_refl : Steps δ1 s1 δ1 s1
-  | step_trans {δ2 δ3 : LocalStore Γ} {s2 s3 : Stm Γ σ} :
-      Step δ1 δ2 s1 s2 -> Steps δ2 s2 δ3 s3 -> Steps δ1 s1 δ3 s3.
+  Inductive Steps {Γ : Ctx (𝑿 * Ty)} {σ : Ty} (γ1 : RegStore) (δ1 : LocalStore Γ) (s1 : Stm Γ σ) : RegStore -> LocalStore Γ -> Stm Γ σ -> Prop :=
+  | step_refl : Steps γ1 δ1 s1 γ1 δ1 s1
+  | step_trans {γ2 γ3 : RegStore} {δ2 δ3 : LocalStore Γ} {s2 s3 : Stm Γ σ} :
+      Step γ1 γ2 δ1 δ2 s1 s2 -> Steps γ2 δ2 s2 γ3 δ3 s3 -> Steps γ1 δ1 s1 γ3 δ3 s3.
 
-  (* Notation "'⟨' δ1 ',' s1 '⟩' '--->' '⟨' δ2 ',' s2 '⟩'" := (@Step _ _ δ1 δ2 s1 s2). *)
-  Notation "'⟨' δ1 ',' s1 '⟩' --->* '⟨' δ2 ',' s2 '⟩'" := (@Steps _ _ δ1 s1 δ2 s2).
+  Notation "⟨ γ1 , δ1 , s1 ⟩ --->* ⟨ γ2 , δ2 , s2 ⟩" := (@Steps _ _ γ1 δ1 s1 γ2 δ2 s2).
 
 End SmallStep.
